Implement mlswg/mls-protocol#837

fstar/treesync/code/MLS.TreeSync.Invariants.UnmergedLeaves.fst
@@ -7,9 +7,30 @@ open MLS.TreeSync.Types
 
 #set-options "--fuel 1 --ifuel 1"
 
+// Check that the unmerged leaf li is in a non-blank leaf in t's subtree
 val unmerged_leaf_exists: #bytes:Type0 -> {|bytes_like bytes|} -> #tkt:treekem_types bytes -> #l:nat -> #i:tree_index l -> treesync bytes tkt l i -> nat -> bool
 let unmerged_leaf_exists #bytes #bl #tkt #l #i t li =
   leaf_index_inside l i li && Some? (leaf_at t li)
+
+// Check that the unmerged leaf li is unmerged everywhere it can be in t's subtree
+val unmerged_leaf_consistent:
+  #bytes:Type0 -> {|bytes_like bytes|} -> #tkt:treekem_types bytes ->
+  #l:nat -> #i:tree_index l ->
+  treesync bytes tkt l i -> nat_lbytes 4 ->
+  bool
+let rec unmerged_leaf_consistent #bytes #bl #tkt #l #i t li =
+  match t with
+  | TLeaf _ -> true
+  | TNode opt_content left right ->
+    (
+      match opt_content with
+      | None -> true
+      | Some content ->
+        // Read as: leaf_index_inside ... ==> List.Tot.mem ...
+        (not (leaf_index_inside l i li)) || (List.Tot.mem li content.unmerged_leaves)
+    ) &&
+    unmerged_leaf_consistent left li &&
+    unmerged_leaf_consistent right li
 
 val unmerged_leaves_sorted: list (nat_lbytes 4) -> bool
 let rec unmerged_leaves_sorted l =
@@ -28,6 +49,7 @@ let rec unmerged_leaves_ok #bytes #bl #tkt #l #i t =
       | None -> true
       | Some content ->
         List.Tot.for_all (unmerged_leaf_exists t) content.unmerged_leaves &&
+        List.Tot.for_all (unmerged_leaf_consistent t) content.unmerged_leaves &&
         unmerged_leaves_sorted content.unmerged_leaves
     in
     content_ok && unmerged_leaves_ok left && unmerged_leaves_ok right
